# Saved by TopBraid on Mon Oct 25 14:03:00 MSD 2010
# baseURI: http://www.w3.org/2001/02/acls/ns

@prefix acls:    <http://www.w3.org/2001/02/acls/ns#> .
@prefix owl:     <http://www.w3.org/2002/07/owl#> .
@prefix rdf:     <http://www.w3.org/1999/02/22-rdf-syntax-ns#> .
@prefix rdfs:    <http://www.w3.org/2000/01/rdf-schema#> .
@prefix xsd:     <http://www.w3.org/2001/XMLSchema#> .

<http://www.w3.org/2001/02/acls/ns>
      rdf:type owl:Ontology .

acls:Group
      rdf:type rdfs:Class ;
      rdfs:comment "Collection of Principles." ;
      rdfs:label "Group" ;
      rdfs:subClassOf acls:Identity .

acls:Identity
      rdf:type rdfs:Class ;
      rdfs:comment "Any entity to which access may be granted to a rdf:resource."^^xsd:string ;
      rdfs:isDefinedBy acls: ;
      rdfs:label "Identity"@en ;
      rdfs:subClassOf rdfs:Resource .

acls:Principle
      rdf:type rdfs:Class ;
      rdfs:comment "An Identity to which credentials or other uniquely distinguishing characteristics may be assigned." ;
      rdfs:label "Principle" ;
      rdfs:subClassOf acls:Identity .

acls:ResourceAccessRule
      rdf:type rdfs:Class ;
      rdfs:comment "An assertion of access privileges to a rdf:resource." ;
      rdfs:isDefinedBy acls: ;
      rdfs:label "Access Rule" .

acls:access
      rdf:type rdf:Property ;
      rdfs:comment "The access privileges extended to an accessor." ;
      rdfs:domain acls:ResourceAccessRule ;
      rdfs:isDefinedBy acls: ;
      rdfs:label "access"@en ;
      rdfs:range rdfs:Literal .

acls:accessor
      rdf:type rdf:Property ;
      rdfs:comment "The rdf:resource identifying an entity (for intance, a user) to whom access privileges have been granted." ;
      rdfs:domain acls:ResourceAccessRule ;
      rdfs:isDefinedBy acls: ;
      rdfs:label "accessor" ;
      rdfs:range acls:Identity .

acls:hasAccessTo
      rdf:type rdf:Property ;
      rdfs:comment "Relates an Access Rule to the rdf:resources to which the rule applies.  The inverse relation is 'accessedBy'" ;
      rdfs:domain acls:ResourceAccessRule ;
      rdfs:isDefinedBy acls: ;
      rdfs:label "has access to" ;
      rdfs:range rdfs:Resource .

acls:time-interval
      rdf:type rdf:Property ;
      rdfs:comment "The time interval over which an ACL rule is declared." ;
      rdfs:domain acls:ResourceAccessRule ;
      rdfs:isDefinedBy acls: ;
      rdfs:label "time interval"@en ;
      rdfs:range rdfs:Literal .
